src/QueryStructure/IndexedEnsembles.v
@@ -1,0 +1,72 @@
+Require Import List String FunctionalExtensionality Ensembles.
+
+Class UnConstrRelationAbsRClass {A B : Type} :=
+  { UnConstrRelationAbsR : Ensemble A -> B -> Prop }.
+
+Section IndexedEnsembles.
+
+  Context {ElementType : Type}.
+
+  Record IndexedElement :=
+    { elementIndex : nat;
+      indexedElement : ElementType }.
+
+  Definition IndexedEnsemble := Ensemble IndexedElement.
+
+  Definition IndexedEnsembleSubtract
+             (element : ElementType)
+             (ens : IndexedEnsemble)
+  : IndexedEnsemble :=
+    fun element' => indexedElement element' <> element /\ ens element'.
+
+  (* 'Deleting' a set of tuples [R] from a relation [F] is the same
+   as taking the intersection of [F] and the complement of [R]. *)
+  Definition EnsembleDelete
+             (F : IndexedEnsemble)
+             (R : Ensemble ElementType)
+    := Intersection _ F (Complement _ (fun iel => R (indexedElement iel))).
+
+  (* Definition IndexedEnsembleUpdate
+             (element : ElementType)
+             (ens : IndexedEnsemble)
+             (cond : Ensemble ElementType)
+             (f : ElementType -> ElementType)
+  : IndexedEnsemble :=
+    fun element' =>
+        indexedElement element' <> element /\ ens element'.
+
+  : Prop := ((fst kv) = k /\ exists v, (snd kv) = f v /\ In _ ens (k, v)) \/
+            (EnsembleRemove k ens kv). *)
+
+  Definition EnsembleListEquivalence
+             {A}
+             (ensemble : Ensemble A)
+             (seq : list A) :=
+    NoDup seq /\
+    forall x, Ensembles.In _ ensemble x <-> List.In x seq.
+
+  Definition UnIndexedEnsembleListEquivalence
+             (ensemble : IndexedEnsemble)
+             (l : list ElementType)  :=
+    exists l', (map indexedElement l') = l /\
+               EnsembleListEquivalence ensemble l'.
+
+  Definition UnConstrFreshIdx
+             (ensemble : IndexedEnsemble)
+             (bound : nat) :=
+  forall element,
+    ensemble element
+    -> lt (elementIndex element) bound.
+
+  Definition EnsembleIndexedListEquivalence
+             (ensemble : IndexedEnsemble)
+             (l : list ElementType) :=
+    (exists bound, UnConstrFreshIdx ensemble bound)
+    /\ UnIndexedEnsembleListEquivalence ensemble l.
+
+  Global Instance EnsembleListEquivalence_AbsR :
+    @UnConstrRelationAbsRClass (IndexedElement)
+                               (list ElementType) :=
+    {| UnConstrRelationAbsR := EnsembleIndexedListEquivalence|}.
+
+End IndexedEnsembles.
