src/QueryStructure/Refinements/Bags/BagADT.v
@@ -1,0 +1,57 @@
+Require Import String Omega List FunctionalExtensionality Ensembles
+        IndexedEnsembles Computation ADT ADTRefinement ADTNotation
+        BuildADTRefinements.
+
+Open Scope string.
+
+Section BagADT.
+
+  Variable ElementType : Type.
+  Variable SearchTermType : Type.
+  Variable SearchTermMatcher : SearchTermType -> ElementType -> bool.
+
+  Definition BagSig : ADTSig :=
+    ADTsignature {
+        Constructor "EmptyCache" : unit             -> rep,
+        Method "Find" : rep x SearchTermType -> rep x list ElementType,
+        Method "Enumerate" : rep x SearchTermType -> rep x list ElementType,
+        Method "Insert"    : rep x ElementType -> rep x unit,
+        Method "Count"     : rep x SearchTermType  -> rep x nat,
+        Method "Delete"    : rep x SearchTermType  -> rep x (list ElementType)
+        (*Method "Update"    : rep x (SearchTermType * UpdateTermType) -> rep x unit *)
+  }.
+
+  Definition BagSpec : ADT BagSig :=
+    ADTRep (@IndexedEnsemble ElementType) {
+        Def Constructor "EmptyCache" (_ : unit) : rep :=
+          ret (Empty_set _),
+
+        Def Method "Find" (r : rep, f : SearchTermType)
+          : list ElementType :=
+            results <- {l | EnsembleIndexedListEquivalence r l};
+        ret (r, filter (SearchTermMatcher f) results),
+
+        Def Method "Enumerate" (r : rep, f : SearchTermType)
+          : list ElementType :=
+            results <- {l | EnsembleIndexedListEquivalence r l};
+        ret (r, results),
+
+        Def Method "Insert" (r : rep, element : ElementType) : unit :=
+          freshIdx <- {freshIdx | UnConstrFreshIdx r freshIdx};
+        ret (Add _ r {| elementIndex := freshIdx;
+                        indexedElement := element |}, ()),
+
+        Def Method "Count" (r : rep, f : SearchTermType) : nat :=
+          results <- {l | EnsembleIndexedListEquivalence r l};
+        ret (r, length (filter (SearchTermMatcher f) results)),
+
+        Def Method "Delete" (r : rep, f : SearchTermType)
+        : list ElementType :=
+          deleted <- {l | EnsembleIndexedListEquivalence r l};
+          ret (EnsembleDelete
+                 r
+                 (fun tup => SearchTermMatcher f tup = true),
+               filter (SearchTermMatcher f) deleted)
+           }.
+
+End BagADT.
