src/QueryStructure/Refinements/EnsembleListEquivalenceProperties.v
@@ -1,4 +1,4 @@
-Require Export EnsembleListEquivalence.
+Require Export IndexedEnsembles.
 Require Import Ensembles List AdditionalPermutationLemmas.
 
 Lemma EnsembleListEquivalence_slice :
@@ -6,12 +6,12 @@ Lemma EnsembleListEquivalence_slice :
     EnsembleListEquivalence ens (a ++ b ++ c) ->
     EnsembleListEquivalence (fun x => ens x /\ ~ List.In x b) (a ++ c).
 Proof.
-  unfold EnsembleListEquivalence, Ensembles.In; simpl; 
+  unfold EnsembleListEquivalence, Ensembles.In; simpl;
   repeat setoid_rewrite in_app_iff; intros * (no_dup & in_seq).
-  split. 
+  split.
   - eapply NoDup_slice; eauto.
   - intros; split.
-    + intros (in_ens & not_in_b); 
+    + intros (in_ens & not_in_b);
       specialize (in_seq x); intuition.
     + intros [ in_a | in_c ]; split; try solve [apply in_seq; intuition];
       apply (NoDup_app_inv' _ _ _ no_dup); intuition.
