src/QueryStructure/Relation.v
@@ -1,17 +1,19 @@
 Require Import List String FunctionalExtensionality Ensembles
-        Common.ilist Common.StringBound Program Schema
-        Heading Tuple.
+        Common.ilist Common.StringBound Program IndexedEnsembles
+        Schema Heading Tuple.
 
 (* A relation is a collection of tuples (described by a proposition)
    which satisfy the schema constraints. *)
 
 Record Relation (RelationSchema : Schema) :=
-  { rel : Ensemble (@IndexedTuple (schemaHeading RelationSchema));
+  { rel : @IndexedEnsemble (@Tuple (schemaHeading RelationSchema));
     constr :
       match (schemaConstraints RelationSchema) with
         | Some Constr =>
          forall tup tup',
-           rel tup -> rel tup' -> Constr tup tup'
+           rel tup 
+           -> rel tup' 
+           -> Constr (indexedTuple tup) (indexedTuple tup')
         | None => True
       end
   }.
@@ -20,7 +22,7 @@ Definition UnConstrRelation (RelationSchema : Heading) :=
   Ensemble (@IndexedTuple RelationSchema).
 
 Definition UnIndexedTupleIn {heading}
-           (rel : Ensemble (@IndexedTuple heading))
+           (rel : @IndexedEnsemble (@Tuple heading))
            (tup : @Tuple heading):=
-  exists n, rel {|tupleIndex := n;
-                  indexedTuple := tup |}.
+  exists n, rel {| elementIndex := n;
+                   indexedElement := tup |}.
